\documentclass{article}
\usepackage{listings}
\usepackage{mathrsfs}
\usepackage[utf8]{inputenc}
\usepackage{amssymb}
\usepackage{lipsum}
\usepackage{amsmath}
\usepackage{fancyhdr}
\usepackage{geometry}
\usepackage{scrextend}
\usepackage[english,german]{babel}
\usepackage{titling}
\setlength{\droptitle}{-3cm}
\usepackage{tikz}
\usepackage{algorithm,algpseudocode}
\usepackage[doublespacing]{setspace}
\usetikzlibrary{datavisualization}
\usetikzlibrary{datavisualization.formats.functions}
\usepackage{polynom}
\usepackage{amsmath}
\usepackage{gauss}
\usepackage{tkz-euclide}
\usetikzlibrary{datavisualization}
\usetikzlibrary{datavisualization.formats.functions}
\author{
Alexander Mattick Kennung: qi69dube\\
Kapitel 1
}
\usepackage{import}
\date{\today}
\geometry{a4paper, margin=2cm}
\usepackage{stackengine}
\parskip 1em
\newcommand\stackequal[2]{%
  \mathrel{\stackunder[2pt]{\stackon[4pt]{=}{$\scriptscriptstyle#1$}}{%
  $\scriptscriptstyle#2$}}
 }
\makeatletter
\renewcommand*\env@matrix[1][*\c@MaxMatrixCols c]{%
  \hskip -\arraycolsep
  \let\@ifnextchar\new@ifnextchar
  \array{#1}}
\makeatother
\lstset{
  language=haskell,
}
\lstnewenvironment{code}{\lstset{language=Haskell,basicstyle=\small}}{}
\usepackage{enumitem}
\setlist{nosep}
\usepackage{titlesec}

\titlespacing*{\subsection}{0pt}{2pt}{3pt}
\titlespacing*{\section}{0pt}{0pt}{5pt}
\titlespacing*{\subsubsection}{0pt}{1pt}{2pt}
\title{Vorlesung 3}


\begin{document}
	\maketitle
	$\sigma_x^n = \sqrt{\frac{1}{n}\sum\limits^n_{i=1} x_i^2-\overline{x}^2}$\\
	Beweis (Ã¼ber varianz, damit man sich die Wurzel mitschleppen sparen kann):\\
	$\sigma_{\overline{x}}^n := (\frac{1}{n}\sum\limits^n_{i=1} x_i^2-\overline{x}^2)^\frac{1}{2}$\\
	$\sigma_{\overline{x}}^n = \frac{1}{n}\sum\limits^n_{i=1} (x_i^2-2x_i\overline{x}+\overline{x}^2)=
	(\frac{1}{n}\sum\limits^n_{i=1}x_i^2-\overline{x}(\frac{2}{n}\sum\limits^n_{i=1}x_i)+\frac{1}{n}\sum\limits^n_{i=1}\overline{x}^2) 
	= (\frac{1}{n}\sum\limits^n_{i=1}x_i^2-\overline{x}(\overline{x}*2)+\overline{x}^2\frac{1}{n}\sum\limits^n_{i=1}1)
	=\frac{1}{n}\sum\limits^n_{i=1}x_i^2-\overline{x}(\overline{x}*2)+\overline{x}^2 =
	 \sum\limits^n_{i=1}x_i^2-\overline{x}^2$

\end{document}